Add some documentation to VC tutorial

src/Lab0/VerifiedVC.v
@@ -3,11 +3,19 @@ Require Import ThreeVariablesAPI.
 
 Module ThreeVarVC (vars : VarsAPI).
 
+  Implicit Types (s:State).
+
   (* note that we need all the weakest preconditions to also talk about return
   values of type [T], so almost everything will take an extra parameter for the
   return type. *)
   Definition t_wp T := forall (k: T -> State -> Prop), (State -> Prop).
 
+  (* this is the core of weakest preconditions: wp k is a precondition that
+     guarantees the postcondition k
+
+     the "weakest" in weakest preconditions means [wp k] is supposed to be the
+     minimal condition necessary to guarantee k, but we don't prove that (as is
+     common) *)
   Definition has_wp T (code: proc T) (wp:t_wp T) :=
     forall (k: T -> State -> Prop),
       proc_spec (fun (_:unit) s0 =>
@@ -21,20 +29,25 @@ Module ThreeVarVC (vars : VarsAPI).
 
   Class quickCode T (code:proc T) : Type :=
     QProc {
-        qc_wp:t_wp T;
-        qc_has_wp: has_wp code qc_wp;
+        (* a quickCode has a _predicate transformer_ function wp that
+        produces a weakest precondition for a given postcondition *)
+        wp: t_wp T;
+        (* ...and this wp is proven correct *)
+        hasWp: has_wp code wp;
       }.
 
-  Arguments qc_wp {T} {code} qc : rename.
-  Arguments qc_has_wp {T} {code} qc : rename.
+  Arguments QProc {T code} wp hasWp.
+  Arguments wp {T} {code} qc : rename.
+  Arguments hasWp {T} {code} qc : rename.
 
   (* the type of QProc is as given in the paper (just written with different
   syntax) *)
-  Check QProc.
+  About QProc.
 
   Instance quick_read var : quickCode (vars.read var).
   Proof.
-    exists (fun k => (fun s => k (StateVar var s) s)).
+    refine (QProc
+              (fun k => (fun s => k (StateVar var s) s)) _).
 
     unfold has_wp; intros.
     step_proc.
@@ -42,11 +55,12 @@ Module ThreeVarVC (vars : VarsAPI).
 
   Instance quick_write var v : quickCode (vars.write var v).
   Proof.
-    exists (fun k => (fun s => k tt (match var with
-                          | VarX => mkState v (StateY s) (StateZ s)
-                          | VarY => mkState (StateX s) v (StateZ s)
-                          | VarZ => mkState (StateX s) (StateY s) v
-                          end))).
+    refine (QProc
+              (fun k => (fun s => k tt (match var with
+                                  | VarX => mkState v (StateY s) (StateZ s)
+                                  | VarY => mkState (StateX s) v (StateZ s)
+                                  | VarZ => mkState (StateX s) (StateY s) v
+                                  end))) _).
 
     unfold has_wp; intros.
     step_proc.
@@ -55,27 +69,41 @@ Module ThreeVarVC (vars : VarsAPI).
 
   Instance quick_ret T (x:T) : quickCode (Ret x).
   Proof.
-    exists (fun k => (fun s => k x s)).
+    refine (QProc
+              (fun k => (fun s => k x s)) _).
 
     unfold has_wp; intros.
     step_proc.
   Defined.
 
+  (* our only notion of code is [proc T], where commands are sequenced with
+  functions rather than being a plain list (the plain list makes more sense for
+  assembly, where there's no notion of "returning" a value)
+
+   For that reason we immediately jump to the "shallow embedding" version in the
+   paper that supports ghost state, although we don't thread ghost state through
+   but return values. *)
   Inductive quickCodes : forall T, proc T -> Type :=
   | QRet : quickCodes (Ret tt)
   | QBind : forall T1 (c:proc T1) T2 (cs:T1 -> proc T2),
-      quickCode c ->
-      (forall x, quickCodes (cs x)) ->
-      quickCodes (Bind c cs)
+      forall (qc:quickCode c)
+        (f_qcs:forall x, quickCodes (cs x)),
+        quickCodes (Bind c cs)
   .
 
+  (* vc_gen is the crux of this approach: it sequences weakest preconditions
+  together from [quickCode] instances to build up all the verification
+  conditions for a whole procedure. *)
   Fixpoint vc_gen T (cs:proc T) (qcs: quickCodes cs) (k: T -> State -> Prop)
            {struct qcs}
     : State -> Prop.
+    (* I had a hard time writing this function so I switched to proof mode. *)
     destruct qcs as [| T1 c T2 cs qc f_qcs]; intro s0.
     - exact (k tt s0).
-    - refine (qc_wp qc _ s0).
-      (* this is vc_gen_Bind cs.tl f_qcs k *)
+    - (* the paper defines an intermediate function; rather than do that, we can
+      just put an _ in Coq and then fill it in as a goal later. *)
+      refine (qc.(wp) _ s0).
+      (* the whole is vc_gen_Bind cs.tl f_qcs k from the paper *)
       intros x s1.
       refine (vc_gen _ (cs x) (f_qcs x) k s1).
   Defined.
@@ -87,40 +115,74 @@ Module ThreeVarVC (vars : VarsAPI).
     induction qcs; simpl.
     - unfold has_wp; step_proc.
     - unfold has_wp in *; intros.
-      pose proof (qc_has_wp q (fun x s1 => vc_gen (cs x) (q0 x) k s1)).
+      (* I started from the paper, but the answer is actually in the goal;
+      alternately, we can rely on Coq to guess the right postcondition for the
+      first procedure *)
+      (* eapply proc_spec_rx; [ eapply (qc_has_wp q) | ]; simplify; eauto. *)
+      pose proof (qc.(hasWp) (fun x s1 => vc_gen (cs x) (f_qcs x) k s1)).
       step_proc.
   Qed.
 
-  Arguments QBind {T1 c T2 cs}.
-
   Definition addX (delta : nat) : proc unit :=
     x <- vars.read VarX;
-    _ <- vars.write VarX (x + delta);
-    Ret tt.
+      _ <- vars.write VarX (x + delta);
+      Ret tt.
+
+  (* we need a quickCodes version of addX to teach the vc generator the
+  structure of the procedure as well as the wp's for all the primitives; here's
+  some magic so Coq will do that for us *)
+  Existing Class quickCodes.
+  Existing Instance QRet.
+  Existing Instance QBind.
+  Arguments QBind {T1 c T2 cs}.
+
+  Definition quick_addX delta : quickCodes (addX delta) := _.
+
+  Theorem quick_addX_is : forall delta,
+      quick_addX delta =
+      (* we could also have written the quickCodes version manually (or from a
+      tool, as in Vale) *)
+      QBind (quick_read VarX)
+            (fun x => QBind (quick_write VarX (x + delta))
+                         (fun _ => QRet)).
+  Proof.
+    reflexivity.
+  Qed.
+
+  Arguments vc_sound {T} cs {qcs}.
 
   Theorem addX_ok : forall delta,
-    proc_spec (fun (_:unit) state => {|
-                   pre := True;
-                   post := fun r state' => state' = mkState (delta + StateX state) (StateY state) (StateZ state);
-                   recovered := fun _ _ => False;
+      proc_spec (fun (_:unit) state => {|
+                     pre := True;
+                     post := fun r state' => state' = mkState (delta + StateX state) (StateY state) (StateZ state);
+                     recovered := fun _ _ => False;
                    |})
-              (addX delta)
-              vars.recover
-              vars.abstr.
+                (addX delta)
+                vars.recover
+                vars.abstr.
   Proof.
     intros.
     spec_intros.
     rename state0 into state.
 
     pose proof
-         (vc_sound (cs:=addX delta)
-                   (QBind (quick_read VarX)
-                          (fun x => QBind (quick_write VarX (x + delta))
-                                       (fun _ => QRet)))
-                   (fun r state' =>
-                      state' =
-                      mkState (delta + StateX state) (StateY state) (StateZ state))).
-    simpl in H0.
+         (vc_sound (addX delta))
+         (fun r state' =>
+            state' =
+            mkState (delta + StateX state) (StateY state) (StateZ state)).
+
+    (* if that's tedious, we could instead get its parts from the goal: *)
+    match goal with
+    | [ |- proc_spec
+            (fun _ state0 =>
+               {| post := @?k0 state0 |})
+            ?code
+            _ _ ] =>
+      let k := constr:(k0 state) in
+      let H := fresh in
+      pose proof (vc_sound code k) as H;
+        simpl in H
+    end.
 
     step_proc.
     f_equal.
